Moved some funcs. Added state induction

poSTVM/poSTVM_alt_inductive.thy
@@ -2,112 +2,11 @@ theory poSTVM_alt_inductive
   imports 
     "~~/poST/poSTVM/poSTVM_state_alt" 
 begin
-datatype statement_result = Break | Continue | Exit | Return | Reset | NextState
+datatype statement_result =  Continue | Exit | Return | NextState
 
-text "Executing unary operation"
-definition unary_op_exec :: "unary_op => basic_post_type \<Rightarrow> basic_post_type" where
-"unary_op_exec op var = (case op of unary_op.Not \<Rightarrow> (basic_post_type_not var) | unary_op.Minus \<Rightarrow> (basic_post_type_minus var))"
 
-text "Executing binary operation"
-definition binary_op_exec :: "binary_op \<Rightarrow> basic_post_type \<Rightarrow> basic_post_type \<Rightarrow> basic_post_type" where
-"binary_op_exec op var1 var2 = 
-  (case op of 
-    binary_op.And \<Rightarrow> basic_post_type.Bool(basic_post_type_and var1 var2)|
- binary_op.Or \<Rightarrow> basic_post_type.Bool(basic_post_type_or var1 var2)|
-    binary_op.Xor \<Rightarrow> basic_post_type.Bool(basic_post_type_xor var1 var2) | 
-    binary_op.Eq \<Rightarrow> basic_post_type.Bool(basic_post_type_or var1 var2)| 
-    binary_op.NotEq \<Rightarrow>basic_post_type.Bool(basic_post_type_noteq var1 var2)| 
-    binary_op.Less \<Rightarrow>basic_post_type.Bool(basic_post_type_less var1 var2)| 
-    binary_op.More \<Rightarrow>basic_post_type.Bool(basic_post_type_more var1 var2)| 
-    binary_op.LessEq \<Rightarrow>basic_post_type.Bool(basic_post_type_lesseq var1 var2)| 
-    binary_op.MoreEq \<Rightarrow>basic_post_type.Bool(basic_post_type_moreeq var1 var2)| 
-    binary_op.Sum \<Rightarrow> basic_post_type_sum var1 var2| 
-    binary_op.Sub \<Rightarrow> basic_post_type_sub var1 var2| 
-    binary_op.Mul \<Rightarrow> basic_post_type_mul var1 var2| 
-    binary_op.Div \<Rightarrow> basic_post_type_div var1 var2| 
-    binary_op.Mod \<Rightarrow> basic_post_type_mod var1 var2)"
-
-datatype stmt = 
-  AssignSt assign_statement |
-  FBInvocation fb_invocation |
-  Return |
-  Exit |
-  ProcessSt process_statement |
-  SetStateSt set_state_statement |
-  ResetSt |
-  IfSt expr stmt stmt |
-  WhileSt expr stmt |
-  Comb stmt stmt |
-  Blank 
 
 value "butlast [1::nat,2,3,4]" 
-
-fun case_list_to_if :: "expr \<Rightarrow> case_list \<Rightarrow> expr" where
-  "case_list_to_if _ [] = expr.Const (const.Bool False)"
-| "case_list_to_if exp [val] = expr.Binary binary_op.Eq exp (expr.Const (const.Nat val))"
-| "case_list_to_if exp (val#other) = 
-    expr.Binary binary_op.Or
-      (expr.Binary binary_op.Eq exp (expr.Const (const.Nat val)))
-      (case_list_to_if exp other)"
-
-
-
-function (sequential) statement_to_stmt :: "statement \<Rightarrow> stmt" and
-        st_list_to_stmt :: "statement list \<Rightarrow> stmt" and
-        if_to_stmt :: "(expr * statement_list) list \<Rightarrow> statement_list option \<Rightarrow> stmt" and
-        case_to_stmt :: "expr \<Rightarrow> (case_list *(statement list)) list \<Rightarrow> statement_list option \<Rightarrow> stmt"where
-  "statement_to_stmt (statement.AssignSt st) = stmt.AssignSt st"
-| "statement_to_stmt (statement.FBInvocation fb) = stmt.FBInvocation fb"
-| "statement_to_stmt (statement.Return) = stmt.Return"
-| "statement_to_stmt (statement.Exit) = stmt.Exit"
-| "statement_to_stmt (statement.ProcessSt st) = stmt.ProcessSt st"
-| "statement_to_stmt (statement.SetStateSt st) = stmt.SetStateSt st"
-| "statement_to_stmt (statement.ResetSt) = stmt.ResetSt"
-| "statement_to_stmt (statement.SelectSt (select_statement.IfSt branches else_option)) =(if_to_stmt branches else_option)"
-| "statement_to_stmt (statement.SelectSt (select_statement.CaseSt exp cases_list else_option)) =(case_to_stmt exp cases_list else_option)"
-| "st_list_to_stmt [] = stmt.Blank"
-| "st_list_to_stmt (st#other) = stmt.Comb (statement_to_stmt st) (st_list_to_stmt other)"
-| "if_to_stmt [] else_option= 
-    (case else_option of
-      None \<Rightarrow> stmt.Blank
-    | Some st_list\<Rightarrow> st_list_to_stmt st_list)"
-| "if_to_stmt (branch#other) else_option =
-    (case branch of (exp,st_list) \<Rightarrow> 
-      stmt.IfSt exp 
-        (st_list_to_stmt st_list) 
-        (if_to_stmt other else_option))"
-| "case_to_stmt exp [] else_option = 
-    (case else_option of
-      None \<Rightarrow> stmt.Blank
-    | Some st_list\<Rightarrow> st_list_to_stmt st_list)"
-| "case_to_stmt exp (cas#other) else_option = 
-    (case cas of (val_list,st_list) \<Rightarrow>
-      stmt.IfSt 
-        (case_list_to_if exp val_list)
-        (st_list_to_stmt st_list)
-        (case_to_stmt exp other else_option))"
-| "statement_to_stmt (statement.IterSt (iter_statement.WhileSt exp st_list)) =
-    stmt.WhileSt exp (st_list_to_stmt st_list)"
-| "statement_to_stmt (statement.IterSt (iter_statement.RepeatSt st_list exp)) =
-    (let body = (st_list_to_stmt st_list) 
-      in stmt.Comb body (stmt.WhileSt exp body))"
-| "statement_to_stmt (statement.IterSt (iter_statement.ForSt var_name (start,end,step_option) st_list)) =
-    stmt.Comb 
-      (stmt.AssignSt (common_var.Symbolic var_name,start))
-      (let cond = expr.Binary binary_op.Less (expr.SymbolicVar var_name) end;
-           body = (st_list_to_stmt st_list);
-           step_st = stmt.AssignSt 
-                      (common_var.Symbolic var_name, 
-                        expr.Binary binary_op.Sum
-                          (expr.SymbolicVar var_name) 
-                          (case step_option of
-                            None \<Rightarrow> expr.Const (const.Nat 1)
-                          | Some step \<Rightarrow> step));
-           new_body = stmt.Comb body step_st
-        in stmt.WhileSt cond new_body)"
-  by pat_completeness auto
-termination by size_change
-
 
 (*
 datatype expr = Unary "unary_op option"  prim_expr |
@@ -140,7 +39,7 @@ inductive
   eval :: "[model_state, expr, basic_post_type] \<Rightarrow> bool" ("_ \<turnstile> _ \<rightarrow> _") and
   exec :: "[statement_result * model_state,stmt,statement_result * model_state] \<Rightarrow> bool" ("_ \<turnstile> _ \<longrightarrow> _")
   where
-    XcptE : "st\<turnstile>exp\<rightarrow>undefined"
+    XcptE : "st\<turnstile>exp\<rightarrow>val"
   | BinOp : "\<lbrakk>st\<turnstile>exp1\<rightarrow>val1;
               st\<turnstile>exp2\<rightarrow>val2;
               val = binary_op_exec bin_op val1 val2 \<rbrakk> \<Longrightarrow>
@@ -207,6 +106,9 @@ inductive
 
 print_theorems
 
+inductive eval_state :: "[model_state,stacked_state,statement_result * model_state] \<Rightarrow> bool" ("_ \<turnstile> _ : _") where
+    XcptState : "st\<turnstile>state:(res,st)"   
+  | Base : "\<lbrakk>(statement_result.Continue,st)\<turnstile>stm\<longrightarrow>(res,st1)\<rbrakk> \<Longrightarrow> st \<turnstile>(name,looped,stm,timeout_op):(res,st1)"
 
 
 (*
