poSTVM/poSTVM_parser_alt.thy
@@ -28,110 +28,97 @@ fun stack_expr :: "expr \<Rightarrow> expr_stack" where
 | "stack_expr (expr.ProcStatEpxr proc_name proc_stat) = [expr_op.CheckProcStat proc_name proc_stat]" 
 | "stack_expr (expr.FunctionCall f_name param_assign_list) = [expr_op.FunctionCall f_name param_assign_list]"
 
-datatype statement_op = 
-  Assign symbolic_var expr_stack |
-  AssignArray symbolic_var expr_stack |
-  FunctionBlockCall func_block_name "param_assign list" |
-  SetPoint point_type |
-  GoPoint point_type |
-  SetState "state_name option" |
-  ProcessStatement "process_name option" process_mod |
-  StatementList "statement_op list" |
-  IfStatement expr_stack |
-  CaseHeadStatement expr_stack |
-  CaseStatement "nat list" |
-  WhileStatement expr_stack |
-  ResetTimer
 
-type_synonym statement_stack = "statement_op list"
+datatype stmt = 
+  AssignSt assign_statement |
+  FBInvocation fb_invocation |
+  Return |
+  Exit |
+  ProcessSt process_statement |
+  SetStateSt set_state_statement |
+  ResetSt |
+  IfSt expr stmt stmt |
+  WhileSt expr stmt |
+  Comb stmt stmt |
+  Blank 
 
-text "Parses nuturals to stack of values"
-definition nat_to_values_stack :: "nat list \<Rightarrow> expr_stack" where
-"nat_to_values_stack nl = (map (\<lambda>val. (expr_op.Value (basic_post_type.Nat val))) nl) "
+value "butlast [1::nat,2,3,4]" 
 
-text "Parses values of basic type tp stack_of_values"
-definition basics_to_values_stack :: "basic_post_type list \<Rightarrow> expr_stack" where
-"basics_to_values_stack bl = (map (\<lambda>val. (expr_op.Value val)) bl)"
+fun case_list_to_if :: "expr \<Rightarrow> case_list \<Rightarrow> expr" where
+  "case_list_to_if _ [] = expr.Const (const.Bool False)"
+| "case_list_to_if exp [val] = expr.Binary binary_op.Eq exp (expr.Const (const.Nat val))"
+| "case_list_to_if exp (val#other) = 
+    expr.Binary binary_op.Or
+      (expr.Binary binary_op.Eq exp (expr.Const (const.Nat val)))
+      (case_list_to_if exp other)"
 
-fun stack_statement :: "statement \<Rightarrow> statement_stack" and
-    stack_statement_list:: "statement list \<Rightarrow>statement_stack" and
-    stack_if_statements :: "(expr * statement_list) list \<Rightarrow> statement_stack" and
-    stack_case_statements :: "(case_list * (statement list)) list \<Rightarrow> statement_stack"  where
-  "stack_statement (statement.AssignSt (var, exp)) = 
-    (case var of 
-      (common_var.Symbolic var_name) \<Rightarrow> [(statement_op.Assign var_name (stack_expr exp))] 
-    | (common_var.Array  var_name exp2) \<Rightarrow>[(statement_op.AssignArray var_name ((stack_expr exp2)@ (stack_expr exp)))])" 
-| "stack_statement (statement.Return) = [statement_op.GoPoint point_type.Return]" 
-| "stack_statement (statement.Exit) = [statement_op.GoPoint point_type.Exit]" 
-| "stack_statement (statement.ProcessSt proc_statement) = 
-  (case proc_statement of
-    process_statement.Start(process_name_option) \<Rightarrow> 
-      [statement_op.ProcessStatement process_name_option process_mod.Restart] |
-    process_statement.Stop(process_name_option) \<Rightarrow>
-      [statement_op.ProcessStatement process_name_option process_mod.Stop] |
-    process_statement.Error(process_name_option) \<Rightarrow> 
-      [statement_op.ProcessStatement process_name_option process_mod.Error])" 
-| "stack_statement (statement.SetStateSt state_name_option) = [statement_op.SetState state_name_option]" 
-| "stack_statement (statement.SelectSt (select_statement.IfSt  if_then_list else_option )) = 
-  (let if_stack = (stack_if_statements if_then_list) in  
-        (case else_option of None \<Rightarrow> if_stack |
-          Some(st_list) \<Rightarrow> if_stack @ (stack_statement_list st_list))
-          @[statement_op.SetPoint point_type.Break])" 
-| "stack_statement_list [] = []" 
-| "stack_statement_list (st#other) = (stack_statement st) @ (stack_statement_list other)" 
-| "stack_if_statements [] = []" 
-| "stack_if_statements (ifs#other) = 
-    (let (exp,st_list) = ifs 
-      in (case st_list of (st_list) \<Rightarrow>  
-            ([statement_op.IfStatement (stack_expr exp)]) 
-            @ [statement_op.StatementList ((stack_statement_list st_list)@ [(statement_op.GoPoint point_type.Break)])]))  
-      @ (stack_if_statements other)" 
-| "stack_statement (statement.SelectSt (select_statement.CaseSt  exp case_then_list else_option)) =
-    (statement_op.CaseHeadStatement (stack_expr exp))
-    #(case else_option of
-        None \<Rightarrow> (stack_case_statements case_then_list)
-      | Some(st_list) \<Rightarrow> (stack_case_statements case_then_list) @ [statement_op.StatementList (stack_statement_list st_list)])
-    @ [statement_op.SetPoint point_type.Break]"
-| "stack_case_statements [] = []"
-| "stack_case_statements (cas#other) =
-    (case cas of
-      (nat_list, st_list) \<Rightarrow>
-        (statement_op.CaseStatement nat_list)
-      # [statement_op.StatementList ((stack_statement_list st_list) @ [(statement_op.GoPoint point_type.Break)])]
-      @ (stack_case_statements other))"
-| "stack_statement (statement.IterSt (iter_statement.ForSt  var_name (exp1,exp2,exp_option) st_list)) = 
-  [statement_op.Assign var_name (stack_expr exp1)] 
-  @ [statement_op.WhileStatement
-      (stack_expr (expr.Binary 
-                    binary_op.LessEq 
-                    (expr.Unary None (expr.SymbolicVar var_name) )
-                    exp2))]
-  @ [statement_op.StatementList 
-      ((stack_statement_list (st_list ))
-      @ [statement_op.Assign 
-          var_name
-          (case exp_option of
-            None \<Rightarrow> [expr_op.Binary binary_op.Sum ,expr_op.Get var_name, expr_op.Value (basic_post_type.Nat 1)] 
-          | Some(exp) \<Rightarrow>[expr_op.Binary binary_op.Sum ,expr_op.Get var_name] @ (stack_expr exp))])] " 
-| "stack_statement (statement.IterSt (iter_statement.WhileSt  exp st_list)) = 
-   [statement_op.WhileStatement (stack_expr exp)]
-   @ [statement_op.StatementList (stack_statement_list st_list)]
-   @ [statement_op.SetPoint point_type.Break]" 
-| "stack_statement (statement.IterSt (iter_statement.RepeatSt  st_list exp)) =  
-    (let st_list = [statement_op.StatementList (stack_statement_list st_list)] 
-    in (st_list
-    @[statement_op.WhileStatement (stack_expr exp)]
-    @ st_list
-    @[statement_op.SetPoint point_type.Break])) " 
-| "stack_statement (statement.ResetSt) = [statement_op.ResetTimer]" 
-| "stack_statement (FBInvocation (fb_name, param_assign_list)) =[statement_op.FunctionBlockCall fb_name param_assign_list]"
 
+
+function (sequential) statement_to_stmt :: "statement \<Rightarrow> stmt" and
+        st_list_to_stmt :: "statement list \<Rightarrow> stmt" and
+        if_to_stmt :: "(expr * statement_list) list \<Rightarrow> statement_list option \<Rightarrow> stmt" and
+        case_to_stmt :: "expr \<Rightarrow> (case_list *(statement list)) list \<Rightarrow> statement_list option \<Rightarrow> stmt"where
+  "statement_to_stmt (statement.AssignSt st) = stmt.AssignSt st"
+| "statement_to_stmt (statement.FBInvocation fb) = stmt.FBInvocation fb"
+| "statement_to_stmt (statement.Return) = stmt.Return"
+| "statement_to_stmt (statement.Exit) = stmt.Exit"
+| "statement_to_stmt (statement.ProcessSt st) = stmt.ProcessSt st"
+| "statement_to_stmt (statement.SetStateSt st) = stmt.SetStateSt st"
+| "statement_to_stmt (statement.ResetSt) = stmt.ResetSt"
+| "statement_to_stmt (statement.SelectSt (select_statement.IfSt branches else_option)) =(if_to_stmt branches else_option)"
+| "statement_to_stmt (statement.SelectSt (select_statement.CaseSt exp cases_list else_option)) =(case_to_stmt exp cases_list else_option)"
+| "st_list_to_stmt [] = stmt.Blank"
+| "st_list_to_stmt (st#other) = stmt.Comb (statement_to_stmt st) (st_list_to_stmt other)"
+| "if_to_stmt [] else_option= 
+    (case else_option of
+      None \<Rightarrow> stmt.Blank
+    | Some st_list\<Rightarrow> st_list_to_stmt st_list)"
+| "if_to_stmt (branch#other) else_option =
+    (case branch of (exp,st_list) \<Rightarrow> 
+      stmt.IfSt exp 
+        (st_list_to_stmt st_list) 
+        (if_to_stmt other else_option))"
+| "case_to_stmt exp [] else_option = 
+    (case else_option of
+      None \<Rightarrow> stmt.Blank
+    | Some st_list\<Rightarrow> st_list_to_stmt st_list)"
+| "case_to_stmt exp (cas#other) else_option = 
+    (case cas of (val_list,st_list) \<Rightarrow>
+      stmt.IfSt 
+        (case_list_to_if exp val_list)
+        (st_list_to_stmt st_list)
+        (case_to_stmt exp other else_option))"
+| "statement_to_stmt (statement.IterSt (iter_statement.WhileSt exp st_list)) =
+    stmt.WhileSt exp (st_list_to_stmt st_list)"
+| "statement_to_stmt (statement.IterSt (iter_statement.RepeatSt st_list exp)) =
+    (let body = (st_list_to_stmt st_list) 
+      in stmt.Comb body (stmt.WhileSt exp body))"
+| "statement_to_stmt (statement.IterSt (iter_statement.ForSt var_name (start,end,step_option) st_list)) =
+    stmt.Comb 
+      (stmt.AssignSt (common_var.Symbolic var_name,start))
+      (let cond = expr.Binary binary_op.Less (expr.SymbolicVar var_name) end;
+           body = (st_list_to_stmt st_list);
+           step_st = stmt.AssignSt 
+                      (common_var.Symbolic var_name, 
+                        expr.Binary binary_op.Sum
+                          (expr.SymbolicVar var_name) 
+                          (case step_option of
+                            None \<Rightarrow> expr.Const (const.Nat 1)
+                          | Some step \<Rightarrow> step));
+           new_body = stmt.Comb body step_st
+        in stmt.WhileSt cond new_body)"
+  by pat_completeness auto
+termination by size_change
+declare statement_to_stmt.simps [simp]
+declare st_list_to_stmt.simps [simp]
+declare if_to_stmt.simps [simp]
+declare case_to_stmt.simps [simp]
 
 text "Stacked version of variables"
 datatype stacked_array_interval = Expr expr_stack expr_stack | Int int int
 datatype stacked_var_init = 
-  Symbolic basic_post_type "expr option" |
-  Array stacked_array_interval "basic_post_type list" "(expr list) option" |
+  Symbolic basic_post_type "expr_stack option" |
+  Array stacked_array_interval "basic_post_type list" "(expr_stack list) option" |
   FunctionBlock func_block_name
 type_synonym stacked_vars = "((symbolic_var, stacked_var_init) fmap)"
 
@@ -152,12 +139,12 @@ definition ainter_to_sainter :: "array_interval \<Rightarrow> stacked_array_inte
     (array_interval.Int val1 val2) \<Rightarrow> (stacked_array_interval.Int val1 val2) |
     (array_interval.Expr exp1 exp2) \<Rightarrow> (stacked_array_interval.Expr (stack_expr exp1) (stack_expr exp2)))"
 
-
+(*
 text "Flattening list of stacks"
 primrec stack_list_to_stack :: "statement_stack list \<Rightarrow> statement_stack" where
 "stack_list_to_stack [] = []" |
 "stack_list_to_stack (st#other) = (st @ (stack_list_to_stack other))"
-
+*)
 text "Converting variable initialization to stacked version"
 definition stack_var_init_decl :: "var_init_decl \<Rightarrow> stacked_var_init" where
 "stack_var_init_decl decl =
@@ -165,12 +152,12 @@ definition stack_var_init_decl :: "var_init_decl \<Rightarrow> stacked_var_init"
     (var_init_decl.Simple (value,exp_option)) \<Rightarrow> 
       (stacked_var_init.Symbolic 
         value 
-        exp_option) |
+        (case exp_option of (Some exp) \<Rightarrow> (Some (stack_expr exp))| None \<Rightarrow> None)) |
     (var_init_decl.Array ((ar_inter,values),array_init_option)) \<Rightarrow> 
       (stacked_var_init.Array 
         (ainter_to_sainter ar_inter) 
         values 
-        array_init_option) |
+        (case array_init_option of (Some ar_init) \<Rightarrow> (Some (map (\<lambda>exp. stack_expr exp) ar_init))| None \<Rightarrow> None)) |
     (var_init_decl.FunctionBlock fb_name) \<Rightarrow> (stacked_var_init.FunctionBlock fb_name))"
 
 text "Converting map of variables to stacked version"
@@ -224,41 +211,67 @@ definition stack_prog_vars :: "program_var list \<Rightarrow> stacked_prog_var l
 "stack_prog_vars pl = (map (\<lambda>val. (stack_prog_var val)) pl)"
 
 text "Stacked version of state declaration"
-datatype timeout = Const const statement_stack | SymbolicVar symbolic_var statement_stack
-type_synonym stacked_state = "state_name * bool * statement_stack * (timeout option)"
+datatype timeout = Const const stmt | SymbolicVar symbolic_var stmt
+type_synonym stacked_state = "state_name * bool * stmt * (timeout option)"
 
 text "Converting state declaration to stacked version"
 fun stack_state :: "state_decl \<Rightarrow> stacked_state" where
 "stack_state (st_name, is_looped, st_list, None) = 
-  (st_name, is_looped, (stack_statement_list st_list), None)" |
+  (st_name, is_looped, (st_list_to_stmt st_list), None)" |
 "stack_state (st_name, is_looped, st_list, (Some (timeout_statement.Const val sl))) = 
-  (st_name, is_looped, (stack_statement_list st_list), (Some (timeout.Const val (stack_statement_list sl))))" |
+  (st_name, is_looped, (st_list_to_stmt st_list), (Some (timeout.Const val (st_list_to_stmt sl))))" |
 "stack_state (st_name, is_looped, st_list, (Some (timeout_statement.SymbolicVar val sl))) = 
-  (st_name, is_looped, (stack_statement_list st_list), (Some (timeout.SymbolicVar val (stack_statement_list sl))))" 
+  (st_name, is_looped, (st_list_to_stmt st_list), (Some (timeout.SymbolicVar val (st_list_to_stmt sl))))" 
+
+primrec get_state_by_name :: "stacked_state list \<Rightarrow> state_name \<Rightarrow> stacked_state" where
+"get_state_by_name (ss#other) name = (let (st_name,_,_,_) = ss in (if st_name = name then ss else (get_state_by_name other name)) )"
+declare get_state_by_name.simps [simp]
+
+primrec get_next_state_sub :: "stacked_state list \<Rightarrow> state_name \<Rightarrow> stacked_state option" where
+  "get_next_state_sub [] _ = None"
+| "get_next_state_sub (ss#other) name = 
+    (let (st_name,_,_,_) = ss in
+      (if st_name = name 
+      then (case other of
+              [] \<Rightarrow> None
+            | (ss1#other) \<Rightarrow> (Some ss1)) 
+      else (get_next_state_sub other name)))"
+declare get_next_state_sub.simps [simp]
+
+definition get_next_state :: "stacked_state list \<Rightarrow> state_name \<Rightarrow> stacked_state" where
+"get_next_state ss_list st_name = 
+  (case (get_next_state_sub ss_list st_name) of 
+    Some st \<Rightarrow> st
+  | None \<Rightarrow> (case ss_list of (st#other) \<Rightarrow> st))" 
+declare get_next_state_def [simp]
+
+definition get_next_state_name :: "stacked_state list \<Rightarrow> state_name \<Rightarrow> state_name" where
+"get_next_state_name ss_list st_name = (fst (get_next_state ss_list st_name))"
+declare get_next_state_name_def [simp]
 
 text "Stacked version of process declaration"
 type_synonym stacked_process = "process_name * stacked_proc_var list * stacked_state list"
 
 text "Converting process declaration to stacked version"
-fun stack_process :: "process_decl \<Rightarrow> stacked_process" where
-"stack_process (p_name, p_var_list, st_decl_list ) =  
-    (p_name, 
+definition stack_process :: "process_decl \<Rightarrow> stacked_process" where
+"stack_process pd =  
+    (let (p_name, p_var_list, st_decl_list ) = pd in (p_name, 
     (stack_proc_vars p_var_list), 
     (map
       (\<lambda>st_decl. stack_state st_decl)
-      st_decl_list))"
+      st_decl_list)))"
 
 text "Stacked version of program declaration"
 type_synonym stacked_program = "program_name * stacked_prog_var list * stacked_process list"
 
 text "Converting program declaration to stacked version"
 fun stack_program :: "program_decl \<Rightarrow> stacked_program" where
-"stack_program (p_name, p_var_list, p_decl_list) =
-  (p_name,
+"stack_program pd =
+  (let (p_name, p_var_list, p_decl_list) = pd in (p_name,
    (stack_prog_vars p_var_list),
    (map
       (\<lambda>p_decl. stack_process p_decl)
-      p_decl_list))"
+      p_decl_list)))"
 
 (*TO DO function block and function stacking*)
 datatype stacked_func_block_var =  
@@ -275,7 +288,7 @@ datatype func_var =
 
 type_synonym stacked_function_block = "func_block_name * stacked_func_block_var list * stacked_process list"
 
-type_synonym stacked_function = "func_name * basic_post_type * func_var list * statement_stack"
+type_synonym stacked_function = "func_name * basic_post_type * func_var list * stmt"
 
 (*TO DO stacking configuration, function blocks and functions*)
 type_synonym stacked_model = "(configuration_decl option) * (global_var_decl list) * (stacked_program list) * (function_block_decl list) * (function_decl list)"
