poSTVM/poSTVM_state_alt.thy
@@ -22,6 +22,7 @@ datatype model_state = ST "(global_var_decl list)"  "((program_name,program_stat
 text "Getting var init from vars map by name"
 definition find_var_by_name :: "symbolic_var  \<Rightarrow>(symbolic_var, stacked_var_init) fmap \<Rightarrow> stacked_var_init option" where
 "find_var_by_name var val =(fmlookup val var) "
+declare find_var_by_name_def [simp]
 
 text "Getting var init from process vars by name"
 primrec get_var_by_name :: "(stacked_proc_var list) \<Rightarrow>  symbolic_var \<Rightarrow>  stacked_var_init option" where
@@ -37,18 +38,20 @@ primrec get_var_by_name :: "(stacked_proc_var list) \<Rightarrow>  symbolic_var 
     in (if res = None 
           then get_var_by_name yz var_name 
           else res))"
-
+declare get_var_by_name.simps [simp]
 print_theorems
 
 text "Getting current process state from program state"
 definition get_cur_proc_state_by_prog :: "program_state \<Rightarrow> process_state" where
 "get_cur_proc_state_by_prog ps = (case (fmlookup (fst (snd ps)) (snd (snd ps))) of Some (st) \<Rightarrow> st)"
+declare get_cur_proc_state_by_prog_def [simp]
 
 text "Getting process vars list in current process from program state"
 definition get_cur_proc_var_list :: "program_state \<Rightarrow>stacked_proc_var list" where 
   "get_cur_proc_var_list ps_state = 
     (let (proc_var_list,st_name,proc_stat,cur_time) = get_cur_proc_state_by_prog ps_state in
       proc_var_list)"
+declare get_cur_proc_var_list_def [simp]
 
 text "Getting current program state from model state"
 definition get_cur_prog_state :: "model_state \<Rightarrow> program_state" where
@@ -57,29 +60,35 @@ definition get_cur_prog_state :: "model_state \<Rightarrow> program_state" where
     (ST global_var_decl_list (ps_map,p_name) function_block_decl_list function_decl_list) \<Rightarrow>
       (case (fmlookup ps_map p_name) of 
         Some(p_state) \<Rightarrow> p_state))"
+declare get_cur_prog_state_def [simp]
 
 text "Getting program state by program name from model state"
 definition get_proc_state_by_prog :: "program_state \<Rightarrow> process_name \<Rightarrow> process_state" where
 "get_proc_state_by_prog ps var_name = (case (fmlookup (fst (snd ps)) var_name) of Some (st) \<Rightarrow> st)"
+declare get_proc_state_by_prog_def [simp]
 
 text "Getting process state by process name from model state" 
 definition get_proc_state :: "model_state \<Rightarrow> process_name \<Rightarrow> process_state" where 
 "get_proc_state st var_name =
   get_proc_state_by_prog (get_cur_prog_state st) var_name"
+declare get_proc_state_def [simp]
 
 text "Getting process vars list of current process of current program from model state"
 definition get_cur_var_list :: "model_state \<Rightarrow> stacked_proc_var list" where
 "get_cur_var_list st = get_cur_proc_var_list (get_cur_prog_state st)"
+declare get_cur_var_list_def [simp]
 
 text "Getting variable init by name from model state"
 definition get_cur_var_by_name :: "model_state \<Rightarrow> symbolic_var \<Rightarrow> stacked_var_init" where
 "get_cur_var_by_name st var_name = the (get_var_by_name (get_cur_var_list st) var_name)"
+declare get_cur_var_by_name_def [simp]
 
 text "Getting symbolic variable value by name from model state"
 definition get_symbvar_by_name :: "model_state \<Rightarrow> symbolic_var \<Rightarrow> basic_post_type" where
 "get_symbvar_by_name st var_name = 
   (case (get_cur_var_by_name st var_name) of
     (stacked_var_init.Symbolic val opt) \<Rightarrow> val)"
+declare get_symbvar_by_name_def [simp]
 
 text "Getting values from list of values"
 definition get_bval_from_list :: "basic_post_type list \<Rightarrow> basic_post_type \<Rightarrow> basic_post_type" where
@@ -87,6 +96,7 @@ definition get_bval_from_list :: "basic_post_type list \<Rightarrow> basic_post_
   (case pos of
     (basic_post_type.Nat val) \<Rightarrow> (nth bl val) |
     (basic_post_type.Int val) \<Rightarrow> (nth bl (nat val)))"
+declare get_bval_from_list_def [simp]
 
 text "Getting array variable single values by name and absolute position from model state"
 definition get_arvar_by_name :: "model_state \<Rightarrow> symbolic_var \<Rightarrow> basic_post_type \<Rightarrow> basic_post_type" where
@@ -94,6 +104,7 @@ definition get_arvar_by_name :: "model_state \<Rightarrow> symbolic_var \<Righta
   (case (get_cur_var_by_name st var_name) of
     (stacked_var_init.Array (stacked_array_interval.Int val1 val2) values  opt) \<Rightarrow>
       (get_bval_from_list values (basic_post_type_sum (basic_post_type.Int val1) pos)))"
+declare get_arvar_by_name_def [simp]
 
 text "Setting in process vars list new var init value by name"
 primrec set_symbvar_in_ps_in_var_list :: "(stacked_proc_var list) \<Rightarrow>  symbolic_var \<Rightarrow> stacked_var_init \<Rightarrow> (stacked_proc_var list)" where
@@ -114,17 +125,20 @@ primrec set_symbvar_in_ps_in_var_list :: "(stacked_proc_var list) \<Rightarrow> 
    stacked_proc_var.OutVar var \<Rightarrow>(stacked_proc_var.OutVar (fmupd var_name value var)) | 
    stacked_proc_var.InOutVar var \<Rightarrow>(stacked_proc_var.InOutVar (fmupd var_name value var)))] @ xs)
 )) "
+declare set_symbvar_in_ps_in_var_list.simps [simp]
 
 text "Setting in process state new var init value by name"
 definition set_symbvar_in_ps :: "process_state \<Rightarrow> symbolic_var \<Rightarrow> stacked_var_init \<Rightarrow> process_state" where
 "set_symbvar_in_ps ps var_name value = 
   (set_symbvar_in_ps_in_var_list (fst ps) var_name value, (fst (snd ps)), (fst (snd (snd ps))), (snd (snd (snd ps))))"
+declare set_symbvar_in_ps_def [simp]
 
 text "Setting in program state in current process new var value by name" 
 definition set_symbvar_in_ps_in_cur_proc :: "program_state \<Rightarrow> symbolic_var \<Rightarrow> stacked_var_init \<Rightarrow> program_state" where
 "set_symbvar_in_ps_in_cur_proc ps var_name value = 
   (case (fmlookup (fst (snd ps)) (snd (snd ps))) of 
     Some(proc_state) \<Rightarrow> ((fst ps), fmupd (snd (snd ps)) (set_symbvar_in_ps proc_state var_name value) (fst (snd ps)), (snd (snd ps))))"
+declare set_symbvar_in_ps_in_cur_proc_def [simp]
 
 text "Setting in model state in current program new var init value by name"
 definition set_symbvar_in_ps_in_cur_prog :: "model_state \<Rightarrow> symbolic_var \<Rightarrow> stacked_var_init \<Rightarrow> model_state" where 
@@ -136,7 +150,7 @@ definition set_symbvar_in_ps_in_cur_prog :: "model_state \<Rightarrow> symbolic_
           (ST global_var_decl_list 
             ((fmupd p_name (set_symbvar_in_ps_in_cur_proc p_state var_name value) ps_map), p_name) 
             function_block_decl_list function_decl_list)))"
-
+declare set_symbvar_in_ps_in_cur_prog_def [simp]
 print_theorems
 
 text "Setting in model state new symbolic var value by name"
@@ -144,13 +158,7 @@ definition set_symbvar :: "model_state \<Rightarrow> symbolic_var \<Rightarrow> 
 "set_symbvar st var_name value =
   (case (get_cur_var_by_name st var_name) of
     (stacked_var_init.Symbolic old_val opt) \<Rightarrow> (set_symbvar_in_ps_in_cur_prog st var_name (stacked_var_init.Symbolic value opt)) )"
-(*
-lemma set_symbvar_part_assoc:
-  "name1 \<noteq> name2 \<Longrightarrow> set_symbvar (set_symbvar st name1 val1) name2 val2 =
-    set_symbvar (set_symbvar st name2 val2) name1 val1"
-  apply (simp add: set_symbvar_def
-                   get_cur_var_by_name_def)
-*)
+declare set_symbvar_def [simp]
 
 text "Setting new val to list in position"
 definition set_bval_to_list :: "basic_post_type list \<Rightarrow> basic_post_type \<Rightarrow> basic_post_type \<Rightarrow> basic_post_type list" where
@@ -158,6 +166,7 @@ definition set_bval_to_list :: "basic_post_type list \<Rightarrow> basic_post_ty
   (case pos of 
     basic_post_type.Nat pos \<Rightarrow> (list_update l pos new_val) |
     basic_post_type.Int pos \<Rightarrow> (list_update l (nat pos) new_val))"
+declare set_bval_to_list_def [simp]
 
 text "Setting in model state new array variable single values by name and absolute position"
 definition set_arvar :: "model_state \<Rightarrow> symbolic_var \<Rightarrow> basic_post_type \<Rightarrow> basic_post_type \<Rightarrow>  model_state" where
@@ -171,12 +180,14 @@ definition set_arvar :: "model_state \<Rightarrow> symbolic_var \<Rightarrow> ba
           (stacked_array_interval.Int val1 val2)
           (set_bval_to_list values (basic_post_type_sum (basic_post_type.Int val1) pos) value)
           opt)) )"
+declare set_arvar_def [simp]
 
 text "Compare process status and estimated status"
 definition check_proc_status :: "model_state \<Rightarrow> process_name \<Rightarrow> proc_status \<Rightarrow> basic_post_type" where
 "check_proc_status st name proc_stat = 
   (let (_,_,_, cur_proc_stat,_) = (get_proc_state st name) 
     in (basic_post_type.Bool (proc_status_is cur_proc_stat proc_stat)))"
+declare check_proc_status_def [simp]
 
 text "Resetting timer in current process in model state"
 definition reset_timer :: "model_state \<Rightarrow> model_state" where
@@ -194,6 +205,7 @@ definition reset_timer :: "model_state \<Rightarrow> model_state" where
                  p_map),p_name)
               pr_map),
             pr_name) fb_list f_list)))"
+declare reset_timer_def [simp]
 
 text "Stopping process by name in model state"
 definition stop_process :: "model_state \<Rightarrow> process_name \<Rightarrow> model_state" where
@@ -217,6 +229,7 @@ definition stop_process :: "model_state \<Rightarrow> process_name \<Rightarrow>
               proc_name) 
             ps_map),
           p_name) function_block_decl_list function_decl_list)))"
+declare stop_process_def [simp]
 
 text "Stopping current process in model state"
 definition stop_same_process :: "model_state  \<Rightarrow> model_state" where
@@ -240,6 +253,7 @@ definition stop_same_process :: "model_state  \<Rightarrow> model_state" where
           p_name) 
         function_block_decl_list 
         function_decl_list)))"
+declare stop_same_process_def [simp]
 
 text "Erroring process by name in model state"
 definition error_process :: "model_state \<Rightarrow> process_name \<Rightarrow> model_state" where
@@ -263,6 +277,7 @@ definition error_process :: "model_state \<Rightarrow> process_name \<Rightarrow
           p_name) 
         function_block_decl_list 
         function_decl_list)))"
+declare error_process_def [simp]
 
 text "Erroring current process in model state"
 definition error_same_process :: "model_state \<Rightarrow> model_state" where
@@ -286,6 +301,7 @@ definition error_same_process :: "model_state \<Rightarrow> model_state" where
           p_name) 
         function_block_decl_list 
         function_decl_list)))"
+declare error_same_process_def [simp]
 
 text "Resetting process by name in model state"
 definition reset_process :: "model_state \<Rightarrow> process_name \<Rightarrow> model_state" where
@@ -309,6 +325,7 @@ definition reset_process :: "model_state \<Rightarrow> process_name \<Rightarrow
           p_name) 
         function_block_decl_list 
         function_decl_list)))"
+declare reset_process_def [simp]
 
 text "Resetting current process in model state"
 definition reset_same_process :: "model_state \<Rightarrow> model_state" where
@@ -332,6 +349,53 @@ definition reset_same_process :: "model_state \<Rightarrow> model_state" where
           p_name) 
         function_block_decl_list 
         function_decl_list)))"
+declare reset_same_process_def [simp]
+
+definition inactive_same_process :: "model_state \<Rightarrow> model_state" where
+"inactive_same_process st =
+(case st of 
+(ST global_var_decl_list (ps_map,p_name) function_block_decl_list function_decl_list) \<Rightarrow>
+(let (var_list,proc_map, proc_name) = (case (fmlookup ps_map p_name) of
+                              Some(p_state) \<Rightarrow> p_state);
+        ((proc_var_list), _,start_st_name, proc_stat, cur_time) = (case (fmlookup proc_map proc_name) of 
+                                    Some(proc_state) \<Rightarrow> proc_state)
+  in (ST 
+        global_var_decl_list 
+        ((fmupd 
+            p_name
+            (var_list,(fmupd 
+                 proc_name
+                 ((proc_var_list), start_st_name,start_st_name, proc_status.Inactive, cur_time)
+                 proc_map), 
+              proc_name) 
+            ps_map),
+          p_name) 
+        function_block_decl_list 
+        function_decl_list)))"
+declare inactive_same_process_def [simp]
+
+definition inactive_process :: "model_state \<Rightarrow> process_name \<Rightarrow> model_state" where
+"inactive_process st target_proc_name =
+   (case st of 
+      (ST global_var_decl_list (ps_map,p_name) function_block_decl_list function_decl_list) \<Rightarrow>
+(let (var_list,proc_map, proc_name) = (case (fmlookup ps_map p_name) of
+                              Some(p_state) \<Rightarrow> p_state);
+        ((proc_var_list), st_name,start_st_name, proc_stat, cur_time) = (case (fmlookup proc_map target_proc_name) of 
+                                    Some(proc_state) \<Rightarrow> proc_state)
+    in (ST 
+        global_var_decl_list 
+        ((fmupd 
+            p_name
+            (var_list,(fmupd 
+                 target_proc_name
+                 ((proc_var_list), st_name,start_st_name, proc_status.Inactive, cur_time)
+                 proc_map), 
+              proc_name) 
+            ps_map),
+          p_name) 
+        function_block_decl_list 
+        function_decl_list)))"
+declare inactive_process_def [simp]
 
 text "Setting new state by name in current process in model state"
 definition set_state :: "model_state \<Rightarrow> state_name \<Rightarrow> model_state" where
@@ -355,6 +419,7 @@ definition set_state :: "model_state \<Rightarrow> state_name \<Rightarrow> mode
           p_name) 
         function_block_decl_list 
         function_decl_list)))"
+declare set_state_def [simp]
 
 text "Extracting new process state from stacked process"
 definition extract_process_state :: "stacked_process \<Rightarrow> process_state" where
@@ -362,7 +427,7 @@ definition extract_process_state :: "stacked_process \<Rightarrow> process_state
   (case sp of 
     (proc_name, var_list,((name, _, _, _)#other)) \<Rightarrow> 
     (var_list, name, name, proc_status.Inactive, (time.Time 0 0 0 0 0)))"
-
+declare extract_process_state_def [simp]
 
 text "Extracting new program state from stacked program"
 definition extract_program_state :: "stacked_program \<Rightarrow> program_state" where 
@@ -376,6 +441,7 @@ definition extract_program_state :: "stacked_program \<Rightarrow> program_state
                             (proc_name,(extract_process_state (proc_name,var_list,state_list)))) 
                           st_proc_list))
     in (var_list,proc_states,name)))"
+declare extract_program_state_def [simp]
 
 text "Extracting new model state from stacked model"
 definition extract_model_state :: "stacked_model \<Rightarrow> model_state" where
@@ -388,6 +454,57 @@ definition extract_model_state :: "stacked_model \<Rightarrow> model_state" wher
       (\<lambda>(name, var_list, proc_list). (name, (extract_program_state (name, var_list, proc_list))))
       prog_list))
   in (model_state.ST global (prog_map,name) fb_list f_list)))"
+declare extract_model_state_def [simp]
 
+fun get_timeout :: "model_state \<Rightarrow> stacked_state \<Rightarrow> time" where
+"get_timeout st ss =
+  (case ss of
+    (_,_,_, Some (timeout.Const t _)) => basic_to_time (const_to_basic t)
+  | (_,_,_, Some (timeout.SymbolicVar var_name _)) => basic_to_time (get_symbvar_by_name st var_name))"
+declare get_timeout.simps [simp]
+
+definition set_timeout :: "model_state \<Rightarrow> timeout \<Rightarrow> model_state" where
+"set_timeout st t = 
+  (case st of (ST global_var_decl_list (ps_map,p_name) function_block_decl_list function_decl_list) \<Rightarrow>
+    (let (var_list,proc_map, proc_name) = (case (fmlookup ps_map p_name) of Some(p_state) \<Rightarrow> p_state);
+        ((proc_var_list),st_name,start_st_name, proc_stat, cur_time) = (case (fmlookup proc_map proc_name) of 
+                                    Some(proc_state) \<Rightarrow> proc_state)
+  in (ST 
+        global_var_decl_list 
+        ((fmupd 
+            p_name
+            (var_list,(fmupd 
+                 proc_name
+                 ((proc_var_list), st_name,start_st_name, proc_status.Timeout (case t of
+                                                                                (timeout.Const t _) \<Rightarrow> basic_to_time (const_to_basic t)
+                                                                              | (timeout.SymbolicVar var_name _) \<Rightarrow> basic_to_time (get_symbvar_by_name st var_name)), cur_time)
+                 proc_map), 
+              proc_name) 
+            ps_map),
+          p_name) 
+        function_block_decl_list 
+        function_decl_list)))"
+declare set_timeout_def [simp]
+
+definition set_timeout_from_state :: "model_state \<Rightarrow> stacked_state \<Rightarrow> model_state" where
+"set_timeout_from_state st ss =
+  (case st of (ST global_var_decl_list (ps_map,p_name) function_block_decl_list function_decl_list) \<Rightarrow>
+    (let (var_list,proc_map, proc_name) = (case (fmlookup ps_map p_name) of Some(p_state) \<Rightarrow> p_state);
+        ((proc_var_list),st_name,start_st_name, proc_stat, cur_time) = (case (fmlookup proc_map proc_name) of 
+                                    Some(proc_state) \<Rightarrow> proc_state)
+  in (ST 
+        global_var_decl_list 
+        ((fmupd 
+            p_name
+            (var_list,(fmupd 
+                 proc_name
+                 ((proc_var_list), st_name,start_st_name, proc_status.Timeout (get_timeout st ss), cur_time)
+                 proc_map), 
+              proc_name) 
+            ps_map),
+          p_name) 
+        function_block_decl_list 
+        function_decl_list)))"
+declare set_timeout_from_state_def [simp]
 
 end
