poST_utils/poST_vars_utils.thy
@@ -6,5 +6,6 @@ definition basics_to_array_interval :: "basic_post_type \<Rightarrow> basic_post
 "basics_to_array_interval var1 var2 = 
   (case (basic_post_type_to_bptint var1,basic_post_type_to_bptint var2) of 
     ((basic_post_type.Int val1), (basic_post_type.Int val2)) \<Rightarrow> array_interval.Int val1 val2)"
+declare basics_to_array_interval_def [simp]
 
 end
